Checkpoint

backend/Asmgenproof0.v
@@ -801,54 +801,126 @@ Variable fn: function.
   Instructions are taken from the first list instead of being fetched
   from memory. *)
 
-Inductive exec_straight: code -> regset -> mem ->
-                         code -> regset -> mem -> Prop :=
+
+(* JT: At first, I wanted to only allow straight execution that do not modify the stack,
+   so I wrote the following function and lemma to capture the fact that some instructions
+   simply increase the PC and cannot jump arbitrarily.
+
+   However, this is mostly useless here, because one can indeed perform a return in a
+   straight-line execution: for instance, in a state where the RA stored on the stack is
+   PC+1, and where the instruction to be executed is SP <- oldSP. 
+ *)
+
+(* Leaving these commented for now*)
+(* Definition straight_instr (i: instruction) := *)
+(*   match i with *)
+(*   (* Unconditional jumps.  Links are always to X1/RA. *) *)
+(*   | Pj_l    _                              (**r jump to label *) *)
+(*   | Pj_s    _ _           (**r jump to symbol *) *)
+(*   | Pj_r    _     _           (**r jump register *) *)
+(*   | Pjal_s  _ _           (**r jump-and-link symbol *) *)
+(*   | Pjal_r  _     _           (**r jump-and-link register *) *)
+
+(*   (* Conditional branches, 32-bit comparisons *) *)
+(*   | Pbeqw   _ _ _            (**r branch-if-equal *) *)
+(*   | Pbnew   _ _ _            (**r branch-if-not-equal signed *) *)
+(*   | Pbltw   _ _ _            (**r branch-if-less signed *) *)
+(*   | Pbltuw  _ _ _            (**r branch-if-less unsigned *) *)
+(*   | Pbgew   _ _ _            (**r branch-if-greater-or-equal signed *) *)
+(*   | Pbgeuw  _ _ _            (**r branch-if-greater-or-equal unsigned *) *)
+(*   (* Conditional branches, 64-bit comparisons *) *)
+(*   | Pbeql   _ _ _            (**r branch-if-equal *) *)
+(*   | Pbnel   _ _ _            (**r branch-if-not-equal signed *) *)
+(*   | Pbltl   _ _ _            (**r branch-if-less signed *) *)
+(*   | Pbltul  _ _ _            (**r branch-if-less unsigned *) *)
+(*   | Pbgel   _ _ _            (**r branch-if-greater-or-equal signed *) *)
+(*   | Pbgeul  _ _ _            (**r branch-if-greater-or-equal unsigned *) *)
+(*   | Pbtbl _ _ *)
+(*     => false *)
+(*   | _ => true *)
+(*   end. *)
+
+(* Lemma straight_instr_increment_pc : *)
+(*   forall i rs1 m1 rs2 m2, *)
+(*     straight_instr i = true -> *)
+(*     exec_instr ge fn i rs1 m1 = Next rs2 m2 -> *)
+(*     rs2#PC = Val.offset_ptr rs1#PC Ptrofs.one. *)
+(* Proof. *)
+(*   intros i rs1 m1 rs2 m2 H0 H1. *)
+(*   destruct i; inv H0; inv H1; simpl; *)
+(*     try (now rewrite nextinstr_pc); *)
+(*     try (now match goal with *)
+(*             | H : exec_load ?ge ?ch ?rs ?m (?rd) ?a ?ofs = Next _ _ |- _ => *)
+(*               unfold exec_load in H; *)
+(*                 destruct (Mem.loadv ch m (Val.offset_ptr (rs a) (eval_offset ge ofs))); *)
+(*                 [inv H; now rewrite nextinstr_pc | congruence] *)
+(*             | H: exec_store ?ge ?ch ?rs ?m ?s ?a ?ofs = Next _ _ |- _ => *)
+(*               unfold exec_store in H; *)
+(*               destruct (Mem.storev ch m (Val.offset_ptr (rs a) (eval_offset ge ofs)) (rs s)); *)
+(*               [inv H; now rewrite nextinstr_pc | congruence] *)
+(*              end); *)
+(*     try now (repeat (match goal with *)
+(*                      | H: (let (m, stk) := ?expr in _) = Next _ _ |- _ => *)
+(*                        destruct expr *)
+(*                      | H: match ?expr with | Some _ => _ | None => _ end = Next _ _ |- _ => *)
+(*                        destruct expr *)
+(*                      | H: Next _ _ = Next _ _ |- _ => inv H; now rewrite nextinstr_pc *)
+(*                      | H: Stuck = Next _ _ |- _ => congruence *)
+(*                      | H: match ?expr with | Vptr _ _ => _ | _ => _ end = _ |- _ => *)
+(*                        destruct expr *)
+(*                      end)). *)
+(* Qed. *)
+
+Inductive exec_straight: stack -> code -> regset -> mem ->
+                         stack -> code -> regset -> mem -> Prop :=
   | exec_straight_one:
-      forall i1 c rs1 m1 rs2 m2,
+      forall i1 s1 c rs1 m1 s2 rs2 m2,
       exec_instr ge fn i1 rs1 m1 = Next rs2 m2 ->
+      forall NEXTSTACK: next_stack i1 s1 rs1 rs2 = s2,
       rs2#PC = Val.offset_ptr rs1#PC Ptrofs.one ->
-      exec_straight (i1 :: c) rs1 m1 c rs2 m2
+      exec_straight s1 (i1 :: c) rs1 m1 s2 c rs2 m2
   | exec_straight_step:
-      forall i c rs1 m1 rs2 m2 c' rs3 m3,
+      forall i s1 c rs1 m1 s2 rs2 m2 s3 c' rs3 m3,
       exec_instr ge fn i rs1 m1 = Next rs2 m2 ->
+      forall NEXTSTACK: next_stack i s1 rs1 rs2 = s2,
       rs2#PC = Val.offset_ptr rs1#PC Ptrofs.one ->
-      exec_straight c rs2 m2 c' rs3 m3 ->
-      exec_straight (i :: c) rs1 m1 c' rs3 m3.
+      exec_straight s2 c rs2 m2 s3 c' rs3 m3 ->
+      exec_straight s1 (i :: c) rs1 m1 s3 c' rs3 m3.
 
 Lemma exec_straight_trans:
-  forall c1 rs1 m1 c2 rs2 m2 c3 rs3 m3,
-  exec_straight c1 rs1 m1 c2 rs2 m2 ->
-  exec_straight c2 rs2 m2 c3 rs3 m3 ->
-  exec_straight c1 rs1 m1 c3 rs3 m3.
+  forall s1 c1 rs1 m1 s2 c2 rs2 m2 s3 c3 rs3 m3,
+  exec_straight s1 c1 rs1 m1 s2 c2 rs2 m2 ->
+  exec_straight s2 c2 rs2 m2 s3 c3 rs3 m3 ->
+  exec_straight s1 c1 rs1 m1 s3 c3 rs3 m3.
 Proof.
   induction 1; intros.
-  apply exec_straight_step with rs2 m2; auto.
-  apply exec_straight_step with rs2 m2; auto.
+  apply exec_straight_step with s2 rs2 m2; auto.
+  apply exec_straight_step with s2 rs2 m2; auto.
 Qed.
 
 Lemma exec_straight_two:
-  forall i1 i2 c rs1 m1 rs2 m2 rs3 m3,
+  forall i1 i2 s1 c rs1 m1 rs2 m2 rs3 m3,
   exec_instr ge fn i1 rs1 m1 = Next rs2 m2 ->
   exec_instr ge fn i2 rs2 m2 = Next rs3 m3 ->
   rs2#PC = Val.offset_ptr rs1#PC Ptrofs.one ->
   rs3#PC = Val.offset_ptr rs2#PC Ptrofs.one ->
-  exec_straight (i1 :: i2 :: c) rs1 m1 c rs3 m3.
+  exec_straight s1 (i1 :: i2 :: c) rs1 m1 (next_stack i2 (next_stack i1 s1 rs1 rs2) rs2 rs3) c rs3 m3.
 Proof.
-  intros. apply exec_straight_step with rs2 m2; auto.
+  intros. apply exec_straight_step with (next_stack i1 s1 rs1 rs2) rs2 m2; auto.
   apply exec_straight_one; auto.
 Qed.
 
 Lemma exec_straight_three:
-  forall i1 i2 i3 c rs1 m1 rs2 m2 rs3 m3 rs4 m4,
+  forall i1 i2 i3 s1 c rs1 m1 rs2 m2 rs3 m3 rs4 m4,
   exec_instr ge fn i1 rs1 m1 = Next rs2 m2 ->
   exec_instr ge fn i2 rs2 m2 = Next rs3 m3 ->
   exec_instr ge fn i3 rs3 m3 = Next rs4 m4 ->
   rs2#PC = Val.offset_ptr rs1#PC Ptrofs.one ->
   rs3#PC = Val.offset_ptr rs2#PC Ptrofs.one ->
   rs4#PC = Val.offset_ptr rs3#PC Ptrofs.one ->
-  exec_straight (i1 :: i2 :: i3 :: c) rs1 m1 c rs4 m4.
+  exec_straight s1 (i1 :: i2 :: i3 :: c) rs1 m1 (next_stack i3 (next_stack i2 (next_stack i1 s1 rs1 rs2) rs2 rs3) rs3 rs4) c rs4 m4.
 Proof.
-  intros. apply exec_straight_step with rs2 m2; auto.
+  intros. apply exec_straight_step with (next_stack i1 s1 rs1 rs2) rs2 m2; auto.
   eapply exec_straight_two; eauto.
 Qed.
 
@@ -856,14 +928,14 @@ Qed.
   (predicate [exec_straight]) correspond to correct Asm executions. *)
 
 Lemma exec_straight_steps_1:
-  forall c rs m c' rs' m',
-  exec_straight c rs m c' rs' m' ->
+  forall s c rs m s' c' rs' m',
+  exec_straight s c rs m s' c' rs' m' ->
   list_length_z (fn_code fn) <= Ptrofs.max_unsigned ->
   forall b ofs,
   rs#PC = Vptr b ofs ->
   Genv.find_funct_ptr ge b = Some (Internal fn) ->
   code_tail (Ptrofs.unsigned ofs) (fn_code fn) c ->
-  plus (step pol) ge (State rs m) E0 (State rs' m').
+  plus (step pol) ge (State s rs m) E0 (State s' rs' m').
 Proof.
   induction 1; intros.
   apply plus_one.
@@ -884,8 +956,8 @@ Proof.
 Qed.
 
 Lemma exec_straight_steps_2:
-  forall c rs m c' rs' m',
-  exec_straight c rs m c' rs' m' ->
+  forall s c rs m s' c' rs' m',
+  exec_straight s c rs m s' c' rs' m' ->
   list_length_z (fn_code fn) <= Ptrofs.max_unsigned ->
   forall b ofs,
   rs#PC = Vptr b ofs ->
@@ -906,37 +978,38 @@ Qed.
 
 (** A variant that supports zero steps of execution *)
 
-Inductive exec_straight_opt: code -> regset -> mem -> code -> regset -> mem -> Prop :=
-  | exec_straight_opt_refl: forall c rs m,
-      exec_straight_opt c rs m c rs m
-  | exec_straight_opt_intro: forall c1 rs1 m1 c2 rs2 m2,
-      exec_straight c1 rs1 m1 c2 rs2 m2 ->
-      exec_straight_opt c1 rs1 m1 c2 rs2 m2.
+Inductive exec_straight_opt: stack -> code -> regset -> mem -> stack -> code -> regset -> mem -> Prop :=
+  | exec_straight_opt_refl: forall c rs m s,
+      exec_straight_opt s c rs m s c rs m
+  | exec_straight_opt_intro: forall s1 c1 rs1 m1 s2 c2 rs2 m2,
+      exec_straight s1 c1 rs1 m1 s2 c2 rs2 m2 ->
+      exec_straight_opt s1 c1 rs1 m1 s2 c2 rs2 m2.
 
 Lemma exec_straight_opt_left:
-  forall c3 rs3 m3 c1 rs1 m1 c2 rs2 m2,
-  exec_straight c1 rs1 m1 c2 rs2 m2 ->
-  exec_straight_opt c2 rs2 m2 c3 rs3 m3 ->
-  exec_straight c1 rs1 m1 c3 rs3 m3.
+  forall s3 c3 rs3 m3 s1 c1 rs1 m1 s2 c2 rs2 m2,
+  exec_straight s1 c1 rs1 m1 s2 c2 rs2 m2 ->
+  exec_straight_opt s2 c2 rs2 m2 s3 c3 rs3 m3 ->
+  exec_straight s1 c1 rs1 m1 s3 c3 rs3 m3.
 Proof.
   destruct 2; intros. auto. eapply exec_straight_trans; eauto. 
-Qed.
+Qed
+.
 
 Lemma exec_straight_opt_right:
-  forall c3 rs3 m3 c1 rs1 m1 c2 rs2 m2,
-  exec_straight_opt c1 rs1 m1 c2 rs2 m2 ->
-  exec_straight c2 rs2 m2 c3 rs3 m3 ->
-  exec_straight c1 rs1 m1 c3 rs3 m3.
+  forall s3 c3 rs3 m3 s1 c1 rs1 m1 s2 c2 rs2 m2,
+  exec_straight_opt s1 c1 rs1 m1 s2 c2 rs2 m2 ->
+  exec_straight s2 c2 rs2 m2 s3 c3 rs3 m3 ->
+  exec_straight s1 c1 rs1 m1 s3 c3 rs3 m3.
 Proof.
   destruct 1; intros. auto. eapply exec_straight_trans; eauto. 
 Qed.
 
 Lemma exec_straight_opt_step:
-  forall i c rs1 m1 rs2 m2 c' rs3 m3,
+  forall i s1 c rs1 m1 rs2 m2 s3 c' rs3 m3,
   exec_instr ge fn i rs1 m1 = Next rs2 m2 ->
   rs2#PC = Val.offset_ptr rs1#PC Ptrofs.one ->
-  exec_straight_opt c rs2 m2 c' rs3 m3 ->
-  exec_straight (i :: c) rs1 m1 c' rs3 m3.
+  exec_straight_opt (next_stack i s1 rs1 rs2) c rs2 m2 s3 c' rs3 m3 ->
+  exec_straight s1 (i :: c) rs1 m1 s3 c' rs3 m3.
 Proof.
   intros. inv H1. 
 - apply exec_straight_one; auto.
@@ -944,11 +1017,11 @@ Proof.
 Qed.
 
 Lemma exec_straight_opt_step_opt:
-  forall i c rs1 m1 rs2 m2 c' rs3 m3,
+  forall i s1 c rs1 m1 rs2 m2 s3 c' rs3 m3,
   exec_instr ge fn i rs1 m1 = Next rs2 m2 ->
   rs2#PC = Val.offset_ptr rs1#PC Ptrofs.one ->
-  exec_straight_opt c rs2 m2 c' rs3 m3 ->
-  exec_straight_opt (i :: c) rs1 m1 c' rs3 m3.
+  exec_straight_opt (next_stack i s1 rs1 rs2) c rs2 m2 s3 c' rs3 m3 ->
+  exec_straight_opt s1 (i :: c) rs1 m1 s3 c' rs3 m3.
 Proof.
   intros. apply exec_straight_opt_intro. eapply exec_straight_opt_step; eauto.
 Qed.
@@ -961,24 +1034,24 @@ Section MATCH_STACK.
 
 Variable ge: Mach.genv.
 
-Inductive match_stack: list Mach.stackframe -> Prop :=
+Inductive match_stack: list Mach.stackframe -> list stackframe -> Prop :=
   | match_stack_nil:
-      match_stack nil
-  | match_stack_cons: forall fb sp ra c s f tf tc,
+      match_stack nil nil
+  | match_stack_cons: forall fb sp ra c s f tf tc s',
       Genv.find_funct_ptr ge fb = Some (Internal f) ->
       transl_code_at_pc ge (Vptr fb ra) fb f c false tf tc ->
       sp <> Vundef ->
-      match_stack s ->
-      match_stack (Stackframe fb sp ra c :: s).
+      match_stack s s' ->
+      match_stack (Mach.Stackframe fb sp ra c :: s) (Stackframe fb ra sp :: s').
 
-Lemma parent_sp_def: forall s, match_stack s -> parent_sp s <> Vundef.
+Lemma parent_sp_def: forall s s', match_stack s s' -> parent_sp s <> Vundef.
 Proof.
   induction 1; simpl.
   unfold Vnullptr; destruct Archi.ptr64; congruence.
   auto.
 Qed.
 
-Lemma parent_ra_def: forall s, match_stack s -> parent_ra s <> Vundef.
+Lemma parent_ra_def: forall s s', match_stack s s' -> parent_ra s <> Vundef.
 Proof.
   induction 1; simpl.
   unfold Vnullptr; destruct Archi.ptr64; congruence.
@@ -986,15 +1059,15 @@ Proof.
 Qed.
 
 Lemma lessdef_parent_sp:
-  forall s v,
-  match_stack s -> Val.lessdef (parent_sp s) v -> v = parent_sp s.
+  forall s s' v,
+  match_stack s s' -> Val.lessdef (parent_sp s) v -> v = parent_sp s.
 Proof.
   intros. inv H0. auto. exploit parent_sp_def; eauto. tauto.
 Qed.
 
 Lemma lessdef_parent_ra:
-  forall s v,
-  match_stack s -> Val.lessdef (parent_ra s) v -> v = parent_ra s.
+  forall s s' v,
+  match_stack s s' -> Val.lessdef (parent_ra s) v -> v = parent_ra s.
 Proof.
   intros. inv H0. auto. exploit parent_ra_def; eauto. tauto.
 Qed.
